Define the global simulation and state adequacy

coq/proof/SimulationLocal.v
@@ -12,10 +12,20 @@ Require Import sflib.
 Require Import paco.
 
 Require Import GenericValues.
-Require Import InvariantMem.
+Require InvMem.
+Require InvState.
 
 Set Implicit Arguments.
 
+
+(* TODO: position *)
+Inductive error_state conf st: Prop :=
+| error_state_intro
+    (STUCK: stuck_state conf st)
+    (NFINAL: s_isFinialState conf st = None)
+.
+
+(* TODO: position *)
 Inductive sInsn_indexed (conf:Config):
   forall (st1 st2:State) (idx1 idx2:nat) (event:trace), Prop :=
 | sInsn_step
@@ -30,15 +40,15 @@ Inductive sInsn_indexed (conf:Config):
 
 Section SimulationLocal.
   Variable (conf_src conf_tgt:Config).
-  Variable (inv0:Relational.t).
+  Variable (inv0:InvMem.Rel.t).
 
   Inductive _sim_local
-            (sim_local: ECStack -> ECStack -> Relational.t -> nat -> State -> State -> Prop)
-            (stack0_src stack0_tgt:ECStack) (inv1:Relational.t) (idx1:nat) (st1_src st1_tgt:State): Prop :=
+            (sim_local: forall (stack0_src stack0_tgt:ECStack) (inv1:InvMem.Rel.t) (idx1:nat) (st1_src st1_tgt:State), Prop)
+            (stack0_src stack0_tgt:ECStack) (inv1:InvMem.Rel.t) (idx1:nat) (st1_src st1_tgt:State): Prop :=
   | _sim_local_error
       st2_src
       (STEP: sop_star conf_src st1_src st2_src E0)
-      (ERROR: stuck_state conf_src st2_src)
+      (ERROR: error_state conf_src st2_src)
 
   | _sim_local_return
       st2_src
@@ -54,11 +64,12 @@ Section SimulationLocal.
       (TYP: typ2_src = typ1_tgt)
       (STACK_SRC: st2_src.(ECS) = stack0_src)
       (STACK_TGT: st1_tgt.(ECS) = stack0_tgt)
-      (MEM: Relational.sem conf_src conf_tgt st2_src.(Mem) st1_tgt.(Mem) inv1)
+      (MEM: InvMem.Rel.sem conf_src conf_tgt st2_src.(Mem) st1_tgt.(Mem) inv1)
       (RET_SRC: getOperandValue conf_src.(CurTargetData) ret2_src st2_src.(EC).(Locals) conf_src.(Globals) = Some retval2_src)
       (RET_TGT: getOperandValue conf_tgt.(CurTargetData) ret1_tgt st1_tgt.(EC).(Locals) conf_tgt.(Globals) = Some retval1_tgt)
-      (RETVAL: GVs.inject inv1.(Relational.inject) retval2_src retval1_tgt)
+      (RETVAL: GVs.inject inv1.(InvMem.Rel.inject) retval2_src retval1_tgt)
 
+  (* TODO: seems duplicate of _sim_local_return. Change semantics? *)
   | _sim_local_return_void
       st2_src
       id2_src
@@ -70,7 +81,7 @@ Section SimulationLocal.
       (TERM_TGT: st1_tgt.(EC).(Terminator) = insn_return_void id1_tgt)
       (STACK_SRC: st2_src.(ECS) = stack0_src)
       (STACK_TGT: st1_tgt.(ECS) = stack0_tgt)
-      (MEM: Relational.sem conf_src conf_tgt st2_src.(Mem) st1_tgt.(Mem) inv1)
+      (MEM: InvMem.Rel.sem conf_src conf_tgt st2_src.(Mem) st1_tgt.(Mem) inv1)
 
   | _sim_local_call
       st2_src
@@ -87,17 +98,17 @@ Section SimulationLocal.
       (VARG: varg2_src = varg1_tgt)
       (FUN_SRC: getOperandValue conf_src.(CurTargetData) fun2_src st2_src.(EC).(Locals) conf_src.(Globals) = Some funval2_src)
       (FUN_TGT: getOperandValue conf_tgt.(CurTargetData) fun1_tgt st1_tgt.(EC).(Locals) conf_tgt.(Globals) = Some funval1_tgt)
-      (FUNVAL: GVs.inject inv1.(Relational.inject) funval2_src funval1_tgt)
+      (FUNVAL: GVs.inject inv1.(InvMem.Rel.inject) funval2_src funval1_tgt)
       (PARAMS_SRC: params2GVs conf_src.(CurTargetData) params2_src st2_src.(EC).(Locals) conf_src.(Globals) = Some args2_src)
       (PARAMS_TGT: params2GVs conf_tgt.(CurTargetData) params1_tgt st1_tgt.(EC).(Locals) conf_tgt.(Globals) = Some args1_tgt)
-      (ARGS: list_forall2 (GVs.inject inv1.(Relational.inject)) args2_src args1_tgt)
-      (MEM: Relational.sem conf_src conf_tgt st2_src.(Mem) st1_tgt.(Mem) inv1)
+      (ARGS: list_forall2 (GVs.inject inv1.(InvMem.Rel.inject)) args2_src args1_tgt)
+      (MEM: InvMem.Rel.sem conf_src conf_tgt st2_src.(Mem) st1_tgt.(Mem) inv1)
       (RETURN:
          forall inv3 mem3_src mem3_tgt retval3_src retval3_tgt
-           (INCR: Relational.le inv1 inv3)
-           (MEM: Relational.sem conf_src conf_tgt mem3_src mem3_tgt inv3)
+           (INCR: InvMem.Rel.le inv1 inv3)
+           (MEM: InvMem.Rel.sem conf_src conf_tgt mem3_src mem3_tgt inv3)
            (RET: noret2_src = false)
-           (RETVAL: GVs.inject inv3.(Relational.inject) retval3_src retval3_tgt),
+           (RETVAL: GVs.inject inv3.(InvMem.Rel.inject) retval3_src retval3_tgt),
          exists idx3,
            sim_local
              stack0_src stack0_tgt inv3 idx3
@@ -118,7 +129,7 @@ Section SimulationLocal.
          exists st2_src st3_src st3_tgt inv3 idx3,
            sop_star conf_src st1_src st2_src E0 /\
            sInsn_indexed conf_src st2_src st3_src idx1 idx3 event /\
-           Relational.le inv1 inv3 /\
+           InvMem.Rel.le inv1 inv3 /\
            sim_local stack0_src stack0_tgt inv3 idx3 st3_src st3_tgt)
   .
   Hint Constructors _sim_local.
@@ -131,10 +142,10 @@ Section SimulationLocal.
     - econs 3; eauto.
     - econs 4; eauto.
       i. exploit RETURN; eauto. i. des.
-      eexists _. splits; eauto.
+      esplits; eauto.
     - econs 5; eauto.
       i. exploit STEP; eauto. i. des.
-      eexists _, _, _, _, _. splits; eauto.
+      esplits; eauto.
   Qed.
   Hint Resolve _sim_local_mon: paco.
 
@@ -164,8 +175,8 @@ Section SimulationLocalFunc.
     forall inv0 stack0_src stack0_tgt mem0_src mem0_tgt
       args_src args_tgt
       ec0_tgt
-      (MEM: Relational.sem conf_src conf_tgt mem0_src mem0_tgt inv0)
-      (ARGS: list_forall2 (GVs.inject inv0.(Relational.inject)) args_src args_tgt)
+      (MEM: InvMem.Rel.sem conf_src conf_tgt mem0_src mem0_tgt inv0)
+      (ARGS: list_forall2 (GVs.inject inv0.(InvMem.Rel.inject)) args_src args_tgt)
       (TGT: init_fdef conf_tgt fdef_tgt args_tgt ec0_tgt),
     exists ec0_src idx0,
       init_fdef conf_src fdef_src args_src ec0_src /\
